compiler/src/ExprImp.v
@@ -11,7 +11,7 @@ Require Import compiler.util.Common.
 Require Import compiler.util.Tactics.
 Require Import compiler.Op.
 Require Import compiler.StateCalculus.
-Require Import compiler.NameWithEq.
+Require Import compiler.Decidable.
 Require Import compiler.Memory.
 
 
