compiler/src/ZName.v
@@ -1,4 +1,0 @@
-Require Import Coq.ZArith.BinInt.
-Require Import compiler.NameWithEq.
-
-Instance ZName: NameWithEq := {| name := Z |}.
